# Lecture 2 (2018-03-20)
- [Proof of natural deduction](#proof-of-natural-deduction)
- [Connectives](#connectives)
  - [Rules for ⋀ (and)](#rule-and)
  - [Rules for ⋁ (or)](#rule-or)
  - [Rules for →](#rule-arrow)
  - [Rules for ¬ (not)](#rule-not)
  - [Rules for ⊥ (bottom/false)](#rule-bottom)
- [Examples](#examples)
  - [#1](#1)
  - [#2](#2)
  - [#3](#3)

## Proof of natural deduction

```java
𝝘 ⊢ 𝞅 // called a sequence
```

There is a proof in natural deduction whichs conclusion is ```𝞅``` and all assumptions belong to ```𝝘```.

1. If ```𝞅 ∈ 𝝘``` then ```𝝘 ⊢ 𝞅```.
2. Suppose ```△ ⊢ ⲯ``` and suppose ```𝝘 ⊢ ∂``` for each ```∂ ∈ △```, then applies ```𝝘 ⊢ ⲯ```.

## Connectives

<a name="rule-and"></a>
### Rules for ⋀ (and)


#### Introduction
```java
 𝞅       ⲯ
----------- ⋀I
   𝞅 ⋀ ⲯ
```

#### Elimination
```java
 𝞅       ⲯ         𝞅       ⲯ
----------- ⋀E    ----------- ⋀E
     𝞅                 ⲯ
```

<a name="rule-or"></a>
### Rules for ⋁ (or)

#### Introduction
```java
     𝞅                 ⲯ
----------- ⋁I    ----------- ⋁I
   𝞅 ⋁ ⲯ             𝞅 ⋁ ⲯ
```

#### Elimination
```java
             𝞅 (1)   ⲯ (2)
             .       .
             .       .
 𝞅 ⋁ ⲯ       𝞂       𝞂
----------------------- ⋁E (1, 2)
             𝞂
```

Compare cases.

<a name="rule-arrow"></a>
### Rules for →

#### Introduction
```java
     𝞅 (1)
     .
     .
     ⲯ
----------- →I (1)
   𝞅 → ⲯ
```

If 𝞅 is a supposition, 𝞅 can be underlined.

#### Elimination
```java
 𝞅       𝞅 → ⲯ
--------------- →E
       ⲯ
```

<a name="rule-not"></a>
### Rules for ¬ (not)

#### Introduction
```java
     𝞅 (1)
     .
     .
     ⊥
----------- ¬I (1)
    ¬𝞅
```

#### Elimination
```java
 𝞅      ¬ⲯ
----------- ¬E
     ⊥
```

<a name="rule-bottom"></a>
### Rules for ⊥ (bottom/false)

#### RAA (Reductio Ad Absurdum)
```java
    ¬𝞅 (1)
     .
     .
     ⊥
----------- RAA (1)
     𝞅
```

## Examples

### #1

#### Question
Solve: ```⊢ (𝞅 → (ⲯ → (𝞅 ⋀ ⲯ)))```

1. Suppose ```𝞅```. We want to show ```(ⲯ → (𝞅 ⋀ ⲯ))```.
2. Suppose ```ⲯ```. We want to show ```(𝞅 ⋀ ⲯ)```.
3. ```→I``` gives us ```(ⲯ → (𝞅 ⋀ ⲯ)```.
4. ```→I``` gives us ```(𝞅 → (ⲯ → (𝞅 ⋀ ⲯ)))```.

#### Answer
```java
 𝞅 (2)   ⲯ (1)
----------- ⋀I
  (𝞅 ⋀ ⲯ)
----------- →I (1)
 (ⲯ → (𝞅 ⋀ ⲯ)
-------------- →I (2)
 (𝞅 → (ⲯ → (𝞅 ⋀ ⲯ)))
```

### #2

#### Question
Solve: ```𝞅 ⋁ ⲯ ⊢ ⲯ ⋁ 𝞅```

#### Answer
```java
              𝞅 (1)         ⲯ (2)
             ------ ⋁I     ------ ⋁I
 𝞅 ⋁ ⲯ       ⲯ ⋁ 𝞅         ⲯ ⋁ 𝞅
---------------------------------- ⋁E (1, 2)
             ⲯ ⋁ 𝞅  
```

### #3

#### Question
Solve: ```⊢ 𝞅 → ¬¬𝞅```

#### Answer
```java
 𝞅 (2)   ¬𝞅 (1)
------------ ¬E
     ⊥
------------ ¬I (1)
    ¬¬𝞅
------------ →I (2)
  𝞅 → ¬¬𝞅
```
